Updating the branch

tests/sparkle_test.c
@@ -1,0 +1,77 @@
+#include <inttypes.h>
+#include <stdio.h>
+#include <stdlib.h>
+#include <string.h>
+#include <sys/types.h>
+#include <sys/stat.h>
+#include <fcntl.h>
+#include <unistd.h>
+#include <time.h>
+#include <stdbool.h>
+#include "test_helpers.h"
+
+#include "Hacl_Impl_Sparkle1.h"
+#include "sparkle_vectors.h"
+
+
+#include <stdint.h>
+#include <string.h>
+#include <stdint.h>
+
+#define ROUNDS 10000
+
+static inline void print(size_t len, uint8_t* comp) {
+  for (size_t i = 0; i < len; i++)
+    printf("%02x",comp[i]);
+  printf("\n");
+}
+
+
+int test()
+{
+    bool ok = true;
+    for (int i = 0; i < sizeof(vectors)/sizeof(sparkle_test_vector); i++)
+    {
+        uint8_t* output_hacl = (uint8_t*) malloc (sizeof (uint8_t) * vectors[i].len);
+        Hacl_Impl_Sparkle1_sparkle256(vectors[i].len, vectors[i].input, output_hacl);
+        ok = ok & compare_and_print(vectors[i].len, output_hacl, vectors[i].output);
+        free(output_hacl);
+    }
+}
+
+void speed()
+{
+    uint8_t* output_hacl = (uint8_t*) malloc (sizeof (uint8_t) * 32);
+    cycles a,b;
+    clock_t t1,t2;
+    for (int j = 0; j < ROUNDS; j++)
+        Hacl_Impl_Sparkle1_sparkle256(1000, output_hacl, output_hacl);
+
+    t1 = clock();
+    a = cpucycles_begin();
+
+    for (int j = 0; j < ROUNDS; j++)
+        Hacl_Impl_Sparkle1_sparkle256(1000, output_hacl, output_hacl);
+    
+    b = cpucycles_end();
+    t2 = clock();
+
+    double timeSparkleOriginal = t2 - t1;
+    double nsigsSparkleOriginal = ((double)ROUNDS) / timeSparkleOriginal;
+    printf("Sparkle PERF \n");
+    printf("Sparkle %f op/s\n",nsigsSparkleOriginal);
+    
+    uint64_t cdiff = b - a;
+    printf("cycles per function call:  %" PRIu64 " \n \n",(uint64_t)cdiff/ROUNDS);
+
+    free(output_hacl);
+}
+
+
+int main(int argc, char const *argv[])
+{
+    test();
+    speed();
+
+	return 0;
+}
